P1.fsti
@@ -180,17 +180,19 @@ val is_balanced (#a: Type) (ptr: t a)
         Spec.is_balanced (v_linked_tree ptr h0) == b))
 
 /// Rebalances a tree according to the comparison function [cmp] on the tree elements
-val rebalance_avl (#a: Type) (cmp:Spec.cmp a) (ptr: t a)
+val rebalance_avl (#a: Type) (ptr: t a)
     : Steel (t a) (linked_tree ptr) (fun ptr' -> linked_tree ptr')
     (requires fun h0 -> True)
     (ensures fun h0 ptr' h1 ->
         Spec.rebalance_avl_wds (v_linked_tree ptr h0) == v_linked_tree ptr' h1)
 
-(*)
 /// Inserts an element [v] in an AVL tree, while preserving the AVL tree invariant
-val insert_avl (#a: Type) (cmp:Spec.cmp a) (ptr: t a) (v: a)
+val insert_avl (#a: Type) (cmp:cmp a) (ptr: t a) (new_data: a)
     : Steel (t a) (linked_tree ptr) (fun ptr' -> linked_tree ptr')
-    (requires fun h0 -> Spec.is_avl cmp (v_linked_tree ptr h0))
+    (requires fun h0 ->
+      Spec.size_of_tree (v_linked_tree ptr h0) < c - 1 /\
+      Spec.is_avl (convert cmp) (v_linked_tree ptr h0))
     (ensures fun h0 ptr' h1 ->
-        Spec.is_avl cmp (v_linked_tree ptr h0) /\
-        Spec.insert_avl cmp (v_linked_tree ptr h0) v == v_linked_tree ptr' h1)
+        Spec.is_avl (convert cmp) (v_linked_tree ptr h0) /\
+        Spec.insert_avl (convert cmp) (v_linked_tree ptr h0) new_data
+        == v_linked_tree ptr' h1)
